did I actually find a sane encoding? look at inductive-type.v

play-with-dependent-types/cpdt-moredep.v
@@ -1,7 +1,16 @@
 (* Solving MoreDep: http://adam.chlipala.net/cpdt/html/MoreDep.html *)
 (* Required to solve dependent type code *)
 Require Import Gt.
+Require Import Arith Bool List Omega.
 
+(* Require Import Cpdt.CpdtTactics Cpdt.MoreSpecif. *)
+
+Require Extraction.
+
+Set Implicit Arguments.
+Set Asymmetric Patterns.
+
+(*
 Definition useGt0 (n: nat) (witness: n > 0) : nat :=
   10.
 
@@ -10,7 +19,6 @@ Definition createGt0 (n : nat) : nat :=
   | O => fun _ => 42
   | S n' => fun E => useGt0 n (eq_ind_r (fun n => n > 0) (gt_Sn_O n') E)
   end eq_refl.
-
 
 Require Import Program.
 
@@ -29,3 +37,51 @@ Proof.
     rewrite E.
     apply gt_Sn_O.
 Defined.
+ *)
+
+
+Section ilist.
+  Variable A : Set.
+
+  Inductive ilist : nat -> Set :=
+  | Nil : ilist O
+  | Cons : forall n, A -> ilist n -> ilist (S n).
+
+
+  Fixpoint app n1 (ls1 : ilist n1) n2 (ls2 : ilist n2) : ilist (n1 + n2) :=
+    match ls1 with
+    | Nil => ls2
+    | Cons _ x ls1' => Cons x (app ls1' ls2)
+    end.
+
+  Fixpoint app' n1 (ls1 : ilist n1) n2 (ls2 : ilist n2) : ilist (n1 + n2) :=
+    match ls1 in (ilist n1) return (ilist (n1 + n2)) with
+    | Nil => ls2
+    | Cons _ x ls1' => Cons x (app' ls1' ls2)
+    end.
+
+
+  Inductive type : Set :=
+  | Nat : type
+  | Bool : type
+  | Prod : type -> type -> type.
+
+  Inductive exp : type -> Set :=
+  | NConst : nat -> exp Nat
+  | Plus : exp Nat -> exp Nat -> exp Nat
+  | Eq : exp Nat -> exp Nat -> exp Bool
+
+  | BConst : bool -> exp Bool
+  | And : exp Bool -> exp Bool -> exp Bool
+  | If : forall t, exp Bool -> exp t -> exp t -> exp t
+
+  | Pair : forall t1 t2, exp t1 -> exp t2 -> exp (Prod t1 t2)
+  | Fst : forall t1 t2, exp (Prod t1 t2) -> exp t1
+  | Snd : forall t1 t2, exp (Prod t1 t2) -> exp t2.
+
+ Fixpoint typeDenote (t : type) : Set :=
+  match t with
+    | Nat => nat
+    | Bool => bool
+    | Prod t1 t2 => typeDenote t1 * typeDenote t2
+  end%type
