program-schedule-encoding/inductive-type.v
@@ -1,0 +1,157 @@
+Require Import Coq.Lists.List.
+Require Import FunInd.
+Require Import Coq.Lists.ListSet.
+Require Import Coq.ZArith.BinInt.
+Require Import Coq.ZArith.BinIntDef.
+Require Import Coq.Numbers.BinNums.
+Require Import Coq.Lists.List.
+Require Import Coq.ZArith.Zbool.
+Require Import Coq.Sorting.Permutation.
+Require Import Coq.Logic.FunctionalExtensionality.
+Require Import Omega.
+Require Import Coq.Bool.Sumbool.
+Require Import Coq.ZArith.Zhints.
+Require Import Coq.Classes.EquivDec.
+Require Import Coq.Structures.Equalities.
+Require Import Coq.FSets.FMapInterface.
+Require Import FMapAVL.
+Require Import FMapFacts.
+Require Import Coq.Logic.FinFun.
+Require Import Nat.
+Require Import VectorDef.
+Require Import MSetWeakList.
+Require Import FSetInterface.
+Require Import FSetList.
+
+(* Require Import CoLoR.Util.FSet.FSetUtil. *)
+(* thank you kind stranger for showing me functorial modules syntax *)
+(* http://newartisans.com/2016/10/using-fmap-in-coq/ *)
+
+Require Import
+  Coq.FSets.FMapList
+  Coq.Structures.OrderedTypeEx.
+
+Module Import M := FMapList.Make(Z_as_OT).
+Module Import MFacts := WFacts(M).
+
+
+
+Require Import
+  Coq.FSets.FMapFacts.
+
+(*Module P := WProperties_fun N_as_OT M.
+*)
+
+
+
+(* An index into memory *)
+Definition memix := nat.
+
+(* values in memory *)
+Definition memvalue := Z.
+
+Inductive write : Type :=
+  Write: memix -> memvalue -> write.
+
+
+Definition memory :=  memix -> memvalue.
+
+Notation "ix '::=' val" := (memory ix val) (at level 60).
+
+(* initial state of memory *)
+Definition initMemory : memory := fun ix => Z0.
+
+Theorem initMemoryAlwaysZero : forall (wix: memix), (initMemory wix) = Z0.
+Proof.
+  auto.
+Qed.
+
+
+Definition writeToMemory (wix: memix) (wval: memvalue) (mold: memory) : memory :=
+  fun ix => if (ix =? wix) then wval else mold ix.
+
+Theorem readFromWriteIdentical : forall (wix: memix) (wval: memvalue) (mem: memory),
+    (writeToMemory wix wval mem) wix = wval.
+Proof.
+  intros wix wval mem.
+  unfold writeToMemory.
+  rewrite Nat.eqb_refl.
+  reflexivity.
+Qed.
+
+
+(* I do not know who Zneq_to_neq fails. TODO: debug this *)
+Theorem readFromWriteDifferent : forall (wix: memix) (rix: memix) (wval : memvalue) (mem: memory),
+    rix <> wix -> (writeToMemory wix wval mem) rix = mem rix.
+Proof.
+  intros wix rix wval mem.
+  intros rix_neq_wix.
+  unfold writeToMemory.
+  assert((rix =? wix) = false).
+  apply Nat.eqb_neq in rix_neq_wix.
+  auto.
+  rewrite H.
+  reflexivity.
+Qed.
+
+
+(* Model the effect of memory writes on memory. *)
+Definition modelWriteSideEffect (mold: memory) (w: write) : memory :=
+  match w with
+  | Write wix wval => (writeToMemory wix wval mold)
+  end.
+
+
+Inductive com: nat ->  Type :=
+| CSeq: forall (n: nat), com n -> write -> com (n + 1)
+| CBegin: com 0.
+
+
+
+Example c_example' : com 2 := (CSeq _ (CSeq _ CBegin (Write 1 100%Z)) (Write 1 100%Z)).
+
+
+Definition timepoint: Type := nat.
+Definition writeset: Type := memix -> list timepoint.
+
+Definition emptyWriteSet : writeset := fun ix => List.nil.
+Definition addToWriteSet (ws: writeset) (ix: memix) (tp: timepoint) : writeset :=
+  fun ix' => if ix' =? ix
+             then List.cons tp (ws ix')
+             else ws ix'.
+Definition singletonWriteSet (ix: memix) (tp: timepoint) : writeset :=
+  addToWriteSet emptyWriteSet ix tp.
+Definition mergeWriteSets (ws ws': writeset) : writeset :=
+  fun ix => ws ix ++ ws' ix.
+               
+
+Definition writeToWriteset (w: write) (tp: timepoint) : writeset :=
+  match w with
+  | Write ix value => singletonWriteSet ix tp
+  end.
+
+  
+Fixpoint computeWriteSet (n: nat) (c: com n) : writeset :=
+  match c with
+  | CSeq n' cs w => mergeWriteSets (computeWriteSet n' cs) (writeToWriteset w n)
+  | CBegin => emptyWriteSet
+  end.
+
+
+Definition dependence: Type := nat * nat.
+Definition dependenceset: Type := list dependence.
+Definition emptydepset : dependenceset := List.nil.
+
+Fixpoint dependencesFromWritesetGo (ws ws': writeset) (t: timepoint) : dependenceset :=
+  match t with
+  | O => emptydepset
+  | S t' => let deps' := dependencesFromWritesetGo ws ws' t' in
+            let w1 := ws t in
+            let w2 := ws' t in
+            deps'
+  end.
+
+Fixpoint computeDependencesGo (prevws: prevWriteSet) (c: com) (tp: timepoint) : dependenceset :=
+  match c with
+  | CWrite write => emptydepset
+  | CSeq c1 c2 => dependencesFromWritesetGo (computeWriteSet )
